deps/poulet4/lib/P4automata/Bisimulations/WPLeapsProofs.v
@@ -7,9 +7,11 @@ Require Import Poulet4.P4automata.P4automaton.
 Require Import Poulet4.FinType.
 Require Import Poulet4.P4automata.ConfRel.
 Require Import Poulet4.Relations.
+Require Import Poulet4.P4automata.WPProofs.
 Require Import Poulet4.P4automata.Bisimulations.Leaps.
+Require Import Poulet4.P4automata.Bisimulations.AlgorithmicLeaps.
+Require Import Poulet4.P4automata.Bisimulations.AlgorithmicLeapsProofs.
 Require Import Poulet4.P4automata.Bisimulations.WPLeaps.
-Require Import Poulet4.P4automata.Bisimulations.AlgorithmicProofs.
 Require Import Poulet4.P4automata.Reachability.
 
 Section WPLeapsProofs.
@@ -32,9 +34,7 @@ Section WPLeapsProofs.
   Context `{H_finite: @Finite (Syntax.H' H) _ H'_eq_dec}.
 
   Variable (a: P4A.t S H).
-
-  Variable (wp: conf_rel a ->
-                list (conf_rel a)).
+  Variable (r: list (state_template a * state_template a)).
 
   Notation conf := (configuration (P4A.interp a)).
 
@@ -47,27 +47,20 @@ Section WPLeapsProofs.
   Notation "R ⊨ S" := (interp_entailment a top {| e_prem := R; e_concl := S |}) (at level 40).
   Notation δ := step.
 
-  Notation "ctx , ⟨ s1 , n1 ⟩ ⟨ s2 , n2 ⟩ ⊢ b" :=
-    ({| cr_st :=
-          {| cs_st1 := {| st_state := s1; st_buf_len := n1 |};
-             cs_st2 := {| st_state := s2; st_buf_len := n2 |}; |};
-        cr_ctx := ctx;
-        cr_rel := b|}) (at level 10).
-  Notation btrue := (BRTrue _ _).
-  Notation bfalse := (BRFalse _ _).
-
   Lemma interp_crel_app:
     forall R1 R2 q1 q2,
       interp_crel a top (R1 ++ R2) q1 q2 <->
       interp_crel a top R1 q1 q2 /\
       interp_crel a top R2 q1 q2.
   Proof.
-  Admitted.
+    intros.
+    induction R1; cbn; intuition.
+    induction R2; intuition.
+  Qed.
 
   Lemma pre_bisimulation_implies_interp_crel:
-    forall R T S q1 q2,
-      pre_bisimulation a wp top R T S ->
-      interp_conf_rel' S q1 q2 ->
+    forall R T q1 q2,
+      pre_bisimulation a (WP.wp r) top R T q1 q2 ->
       top q1 q2 ->
       interp_crel a top (T ++ R) q1 q2.
   Proof.
@@ -87,28 +80,93 @@ Section WPLeapsProofs.
       intuition.
   Qed.
 
-  Lemma pre_bisimulation_implies_equally_accepting:
-    forall S q1 q2 s1 s2,
-      pre_bisimulation a wp top []
-        (mk_init _ _ _ _ (length (valid_state_pairs a)) s1 s2) S ->
-      interp_conf_rel' S q1 q2 ->
+  Lemma interp_rels_vs_interp_crel:
+    forall q1 q2 R,
+      interp_rels top (map (interp_conf_rel a) R) q1 q2 <->
+      interp_crel a top R q1 q2.
+  Proof.
+    induction R; intuition.
+  Qed.
+
+  Lemma pre_bisimulation_embed:
+    forall R T q1 q2,
+      pre_bisimulation a (WP.wp r) top R T q1 q2 ->
+      AlgorithmicLeaps.pre_bisimulation
+        (P4A.interp a)
+        top
+        (map (interp_conf_rel a) R)
+        (map (interp_conf_rel a) T)
+        q1 q2.
+  Proof.
+    intros.
+    induction H0.
+    - apply AlgorithmicLeaps.PreBisimulationClose.
+      now rewrite interp_rels_vs_interp_crel.
+    - apply AlgorithmicLeaps.PreBisimulationSkip.
+      + intros.
+        destruct H0; [|contradiction].
+        rewrite interp_rels_vs_interp_crel in H3.
+        now apply i.
+      + apply IHpre_bisimulation.
+    - eapply AlgorithmicLeaps.PreBisimulationExtend.
+      + intro.
+        destruct H0; [contradiction|].
+        apply n.
+        unfold interp_entailment; simpl; intros.
+        apply H4.
+        now rewrite interp_rels_vs_interp_crel.
+      + fold (map (interp_conf_rel a) T).
+        rewrite map_cons, map_app in IHpre_bisimulation.
+        exact IHpre_bisimulation.
+      + intros.
+        rewrite interp_rels_vs_interp_crel in H4.
+        eapply wp_safe; auto.
+        rewrite <- H2.
+        exact H4.
+  Qed.
+
+  Lemma interp_rels_intersect_top:
+    forall q1 q2 R,
+      interp_rels top R q1 q2 <->
+      (top ⊓ interp_rels top R) q1 q2.
+  Proof.
+    induction R; cbn; intuition.
+  Qed.
+
+  Lemma init_vs_accepting:
+    forall (q1 q2: conf) s1 s2,
+      ⟦mk_init _ _ _ _ (length (valid_state_pairs a)) s1 s2⟧ q1 q2 ->
       top q1 q2 ->
       (accepting q1 <-> accepting q2).
   Proof.
   Admitted.
 
   Lemma wp_leaps_implies_bisim_leaps:
-    forall S q1 q2 s1 s2,
-      pre_bisimulation a wp top []
-        (mk_init _ _ _ _ (length (valid_state_pairs a)) s1 s2) S ->
-      interp_conf_rel' S q1 q2 ->
+    forall q1 q2 s1 s2,
+      let init := mk_init _ _ _ _ (length (valid_state_pairs a)) s1 s2 in
+      pre_bisimulation a (WP.wp r) top [] init q1 q2 ->
       top q1 q2 ->
       bisimilar_with_leaps (P4A.interp a) q1 q2.
   Proof.
-    intros; cofix C; constructor.
-    - eapply pre_bisimulation_implies_equally_accepting;
-      [exact H0 | auto | auto].
-    - (* Guarded. *)
-  Abort.
+    intros.
+    apply AlgorithmicLeapsProofs.algorithmic_leaps_implies_bisimilar_leaps
+    with (R := []) (T := map (interp_conf_rel a) init) (top := top).
+    - simpl interp_rels at 1.
+      unfold coaccepting; intros.
+      erewrite init_vs_accepting.
+      + reflexivity.
+      + rewrite <- interp_rels_vs_interp_crel, interp_rels_intersect_top.
+        exact H2.
+      + destruct H2; apply H2.
+    - simpl interp_rels at 1.
+      unfold follow_closed; intros.
+      clear H2; induction bs using rev_ind.
+      + autorewrite with follow; intuition.
+      + repeat rewrite follow_append.
+        apply top_closed.
+        apply IHbs.
+    - replace [] with (map (interp_conf_rel a) []) by reflexivity.
+      now apply pre_bisimulation_embed.
+  Qed.
 
 End WPLeapsProofs.
